thys/Collections/Lib/Diff_Array.thy
@@ -5,7 +5,7 @@ theory Diff_Array imports
   "~~/src/HOL/Library/Code_Target_Numeral"
 begin
 
-datatype 'a array = Array "'a list"
+datatype_new 'a array = Array "'a list"
 
 subsection {* primitive operations *}
 
